Some notes from enum parsing extraction

examples/kv_parsing/EnumParsing.fst
@@ -205,6 +205,9 @@ let check_length (len:U32.t) (input:bslice) : Pure bool
   (requires True)
   (ensures (fun r -> r ==> U32.v input.len >= U32.v len)) = U32.lte len input.len
 
+val validate_Nothing : stateful_validator (hide (parser_forget parse_Nothing))
+let validate_Nothing = fun input -> Some 0ul
+
 val validate_OneNum : stateful_validator (hide (parser_forget parse_OneNum))
 let validate_OneNum = fun input ->
   if check_length 4ul input then Some 4ul else None
@@ -213,9 +216,13 @@ val validate_TwoNums : stateful_validator (hide (parser_forget parse_TwoNums))
 let validate_TwoNums = fun input ->
   if check_length 8ul input then Some 8ul else None
 
+// this function returns a pointer to a global function; probably better to do
+// this inline than go through a function pointer
+// XXX: these qualifiers don't get the right inlining into validate_numbers, which also has an and_check
+// inline_for_extraction [@"substitute"]
 let validate_numbers_data (t:numbers_tag) : stateful_validator (hide (parse_numbers_data t)) =
   if U8.eq t 0uy then
-    (fun input -> Some 0ul) <: stateful_validator (hide (parser_forget parse_Nothing))
+    validate_Nothing
   else if U8.eq t 1uy then
     validate_OneNum
   else validate_TwoNums
@@ -230,6 +237,7 @@ let coerce_validator #t (#p: parser t)
 
 #reset-options "--z3rlimit 15"
 
+inline_for_extraction [@"substitute"]
 val and_check (#t:Type) (#t':Type) (p: parser t) (p': t -> parser t') (p_st: parser_st (hide p))
               (v: x:t -> stateful_validator (hide (p' x)))
               : stateful_validator (hide (p `and_then` p'))
@@ -246,7 +254,13 @@ let and_check #t #t' p p' p_st v =
 #reset-options
 
 let validate_numbers : stateful_validator (hide parse_numbers) =
-    // XXX: parse_numbers_tag is not inferred from the type of parse_numbers_tag_st
+    // XXX: parse_numbers_tag is not inferred from the type of
+    // parse_numbers_tag_st
+
+    // XXX: validate_numbers_data is legitimately used to get a function
+    // pointer, but KreMLin doesn't keep track of the fact that it's curried and
+    // requires a different application in C (validate_numbers_data(tag)(input)
+    // vs validate_numbers_data(tag, input)).
     and_check parse_numbers_tag parse_numbers_data parse_numbers_tag_st validate_numbers_data
 
 (*! Encoder (pure serialization) *)
